\documentclass[10pt,a4paper]{book}
\usepackage{graphicx}
% Requires \usepackage{graphicx}

\begin{document}
\small

\begin{flushright}
\textsf{\textbf{Context-free Grammar $|$ 323}}
\end{flushright}

\begin{flushleft}
  iii) The finite automata obtained from the expression in step II is
\end{flushleft}

\begin{figure}[h]
  \centering
  % Requires \usepackage{graphicx}
  \includegraphics[width=10cm]{1.1}\\
\end{figure}

\begin{flushleft}
  iv) The constructed right linear grammar is
  
  \qquad
  
  \qquad\qquad\qquad\qquad\qquad\qquad\qquad\qquad\qquad A → 0B,
  
  \qquad\qquad\qquad\qquad\qquad\qquad\qquad\qquad\qquad A → 1E/1
  
  \qquad\qquad\qquad\qquad\qquad\qquad\qquad\qquad\qquad B → 0C
  
  \qquad\qquad\qquad\qquad\qquad\qquad\qquad\qquad\qquad C → 0D/0C
  
  \qquad\qquad\qquad\qquad\qquad\qquad\qquad\qquad\qquad D → 1E/1
  
  \qquad
  
   Here, E is a useless symbol. Eliminate all productions of E. The new productions are
   
   \quad
   
\qquad\qquad\qquad\qquad\qquad\qquad\qquad\qquad\qquad A → 0B

\qquad\qquad\qquad\qquad\qquad\qquad\qquad\qquad\qquad A → 1

\qquad\qquad\qquad\qquad\qquad\qquad\qquad\qquad\qquad B → 0C

\qquad\qquad\qquad\qquad\qquad\qquad\qquad\qquad\qquad C → 0D/0C

\qquad\qquad\qquad\qquad\qquad\qquad\qquad\qquad\qquad D → 1

\qquad

v) Reversing the right side of each production of the right linear grammar,

\qquad

\qquad\qquad\qquad\qquad\qquad\qquad\qquad\qquad\qquad A → B0/1

\qquad\qquad\qquad\qquad\qquad\qquad\qquad\qquad\qquad B → C0

\qquad\qquad\qquad\qquad\qquad\qquad\qquad\qquad\qquad C → D0/C0

\qquad\qquad\qquad\qquad\qquad\qquad\qquad\qquad\qquad D → 1

\qquad

This is the equivalent left linear grammar to the right linear grammar.
\end{flushleft}

\begin{flushleft}
\begin{figure}[h]
  % Requires \usepackage{graphicx}
  \includegraphics[width=3.5cm]{1.2}\\ Convert the following left linear grammar to right linear grammar.
  
  \qquad\qquad\qquad\qquad\qquad S → S10/A1
  
  \qquad\qquad\qquad\qquad\qquad A → A00/00
  
  \textbf{\textsf{Solution:}}
  
  \quad i) Reversing the right side of every production, we get
  
  \qquad\qquad\qquad\qquad\qquad S → 01S/1A
  
  \qquad\qquad\qquad\qquad\qquad A → 00A/00
\end{figure}
  
\end{flushleft}

\end{document}
