\documentclass [12pt]{beamer}
\usepackage{xcolor}	
\usepackage{tikz}
\usetheme{Warsaw}
\useoutertheme{infolines}
\usepackage{ragged2e}
\usepackage{amsmath}
\usepackage{amssymb}
\begin{document}

\section*{mesal 6.33 , 6.34 }
\subsection*{mohamad bahrami nezhad  }	
\begin{frame}
\justifying
Example 6.33  Remove the $\in$ production from the following grammar.
$$
\begin{array}{l}
	\mathrm{S} \rightarrow \mathrm{aS} / \mathrm{A} \\
	\mathrm{A} \rightarrow \mathrm{aA}/\in
\end{array}
$$
\textbf{Solution:} In the previous grammar, there is a null production $\mathrm{A} \rightarrow \in .$ But in the language set generated by the grammar, there is a null string which can be generated by the following way $\mathrm{S} \rightarrow \mathrm{A} \rightarrow \in$. As null string is in the language set, and so the null production cannot be removed from the grammar.
\end{frame}

\begin{frame}

Example 6.34 Convert the following linear grammar into Regular Grammar.
$$
\begin{array}{l}
	\mathrm{S} \rightarrow \text { baS/aA } \\
	\mathrm{A} \rightarrow \mathrm{bbA} / \mathrm{bb}
\end{array}
$$
\textbf{Solution:} Consider two non-terminals $\mathrm{B}$ and $\mathrm{C}$ with production $\mathrm{B} \rightarrow \mathrm{aS}$ and $\mathrm{C} \rightarrow \mathrm{bA} .$ The grammar becomes
$$
\begin{array}{l}
	\mathrm{S} \rightarrow \mathrm{bB} / \mathrm{aA} \\
	\mathrm{A} \rightarrow \mathrm{bC} / \mathrm{bb} \\
	\mathrm{B} \rightarrow \mathrm{aS} \\
	\mathrm{C} \rightarrow \mathrm{bA}
\end{array}
$$
\end{frame}

\begin{frame}
Still the production $\mathrm{A} \rightarrow \mathrm{bb}$ is not a regular grammar. Replace $\mathrm{b}$ by a non-terminal $\mathrm{D}$ with production $\mathrm{D} \rightarrow \mathrm{b}$. The grammar becomes
$$
\begin{array}{l}
	\mathrm{S} \rightarrow \mathrm{bB} / \mathrm{aA} \\
	\mathrm{A} \rightarrow \mathrm{bC} / \mathrm{bD} \\
	\mathrm{B} \rightarrow \mathrm{aS} \\
	\mathrm{C} \rightarrow \mathrm{bA} \\
	\mathrm{D} \rightarrow \mathrm{b}
\end{array}
$$
Now the grammar is regular. For a left linear grammar, there exists a right linear grammar and vice versa. Grammar in one form can be converted into another form. The following section describes the process of conversion.

\end{frame}
\end{document}
